Executable version of root_poly' with correctness added

Root_Power_Poly_Finite_Field.thy
@@ -1,6 +1,6 @@
 theory Root_Power_Poly_Finite_Field
 
-imports "Berlekamp_Zassenhaus.Finite_Field_Factorization" KZG_Def
+imports "Berlekamp_Zassenhaus.Finite_Field_Factorization" 
 "Mason_Stothers.Mason_Stothers"
 
 begin
@@ -47,81 +47,116 @@ proof -
  then show ?thesis unfolding root_poly'_def by (subst Abs_poly_inverse)(auto)
 qed
 
-(*
+lemma root_poly'_0 [simp]: "root_poly' n 0 = 0" 
+unfolding root_poly'_def using zero_poly.abs_eq by auto
+
 text \<open>We also need an executable version of the root poly function.\<close>
-definition root_poly'_impl :: "nat \<Rightarrow> 'a :: zero list \<Rightarrow> 'a list" where
-"root_poly'_impl n cs = nths cs {i. n dvd i \<and> i<length cs}"
-(*
+fun root_poly'_impl :: "nat \<Rightarrow> 'a :: zero list \<Rightarrow> 'a list" where
   "root_poly'_impl n [] = []" |
-  "root_poly'_impl n (c # cs) = (if n dvd (length cs + 1) 
+  "root_poly'_impl n (c # cs) = (if n dvd length cs
       then c#(root_poly'_impl n cs) else root_poly'_impl n cs)"
-*)
 
-lemma root_poly'_code [code]:
+lemma length_root_poly'_impl_null:
+"length (root_poly'_impl n []) = 0"
+by auto
+
+lemma length_root_poly'_impl:
 assumes "n>1"
-shows "coeffs (root_poly' n p) = root_poly'_impl n (coeffs p)"
-proof (rule coeffs_eqI, goal_cases)
-  case (1 m)
-  then show ?case sorry
+shows"length (root_poly'_impl n cs) = 
+  (if n dvd length cs then length cs div n else Suc (length cs div n))" 
+by (induct cs) (auto simp add: div_Suc)
+
+lemma root_poly'_imple_one_elem:
+assumes "n>1"
+shows "root_poly'_impl n [a] = [a]"
+by auto
+
+lemma root_poly'_impl_nth_length:
+assumes "n>1" "m*n < length cs"
+shows "(root_poly'_impl n cs) ! (length (root_poly'_impl n cs) - Suc m) = cs ! (length cs - Suc (m*n))"
+using assms(2) proof (induct cs)
+  case Nil
+  then show ?case by auto
 next
-  case 2
-  then show ?case unfolding root_poly'_impl_def sorry
+  case (Cons a cs)
+  have "(a # root_poly'_impl n cs) ! (length (root_poly'_impl n cs) - m) =
+    (a # cs) ! (length cs - m * n)" if "n dvd length cs" using that Cons assms(1)
+    by (smt (verit, best) Suc_mult_cancel1 bot_nat_0.not_eq_extremum diff_Suc_eq_diff_pred 
+      diff_commute diff_mult_distrib dvd_div_mult_self length_root_poly'_impl mult.commute 
+      nat_neq_iff nonzero_mult_div_cancel_right not_less_eq nth_Cons_0 nth_Cons_pos zero_less_diff)
+  moreover have "root_poly'_impl n cs ! (length (root_poly'_impl n cs) - Suc m) =
+    (a # cs) ! (length cs - m * n)" if "\<not> n dvd length cs" 
+  proof -
+    have not_eq: "length cs \<noteq> m*n" using that by auto
+    then have less: "m * n < length cs" using Cons(2) by auto
+    have "\<not> length cs - m * n = 0" 
+    proof (rule ccontr)
+      assume "\<not> length cs - m * n \<noteq> 0" 
+      then have "length cs \<le> m*n" by simp
+      then show False using Cons not_eq by auto
+    qed
+    then show ?thesis unfolding Cons(1)[OF less] nth_Cons' using that assms by auto
+  qed
+  ultimately show ?case by auto
 qed
-*)
 
+lemma root_poly'_impl_nth:
+assumes "n>1" "m < length (root_poly'_impl n cs)"
+shows "(root_poly'_impl n cs) ! m = cs ! (length cs - Suc ((length (root_poly'_impl n cs) - Suc m)*n))"
+proof -
+  let ?l = "length (root_poly'_impl n cs)"
+  have ass: "(length (root_poly'_impl n cs) - Suc m)*n < length cs" using assms 
+  by (smt (verit, ccfv_threshold) diff_less div_mult_self_is_m dvd_triv_right length_root_poly'_impl 
+    less_Suc_eq_le less_eq_div_iff_mult_less_eq nless_le order_le_less_trans zero_less_Suc)
+  have *: "?l - Suc (?l - Suc m) = m" by (subst Suc_diff_Suc[OF \<open>m<?l\<close>], intro diff_diff_cancel) 
+    (use assms(2) in \<open>auto\<close>)
+  show ?thesis unfolding root_poly'_impl_nth_length[OF assms(1) ass, symmetric] unfolding * by auto
+qed
 
-
-(*
-(*
-coeffs p = [p_0,...,p_r]
-rev (coeffs p) = [p_r,...,p_0]
-root_poly'_impl geht über rev (coeffs p) weil es immer coeff vom nächsthöchsten Grad anschaut
-
-coeffs (root_poly' p) = [p0, pn, p2n,...pmn]
-
-root_poly'_impl n (rev (coeffs p)) = [pmn, ... p2n, pn, p0]
-*)
-
-lemma root_poly'_code [code]:
+text \<open>Correctness of code implementation.\<close>
+(*Lemma for [code]*)
+lemma root_poly'_code:
 assumes "n>1"
-shows "coeffs (root_poly' n p) = root_poly'_impl n (coeffs p)"
+shows "coeffs (root_poly' n p) = strip_while ((=) 0) (rev (root_poly'_impl n (rev (coeffs p))))"
 proof (rule coeffs_eqI, goal_cases)
   case (1 m)
   have *: "poly.coeff (root_poly' n p) m = poly.coeff p (m*n)" by (rule coeff_root_poly'[OF assms])
-  show ?case unfolding * root_poly'_impl_def nths_def apply auto
+  have p0: ?case if "p =0" using that by auto
 
- proof (induction "rev (coeffs p)" arbitrary: p)
-    case Nil
-    then have "p = 0" using coeffs_eq_Nil by fastforce
-    then show ?case unfolding coeff_root_poly'[OF assms] 1 by auto
-  next
-    case (Cons p_deg cs) (* cs = [p_deg-1,... p0] *)
-    define p' where "p' = "
-
-    have "cs = rev (coeffs p')" sorry
-      (* p = p' + x^(deg p) * p_deg*)
-    have "poly.coeff p (m * n) = nth_default 0 (rev (root_poly'_impl n cs)) m" 
-      if "\<not> n dvd length cs + 1"
-    proof -
-      have "rev (coeffs p') = cs"  sorry
-      show ?thesis using nth_default_coeffs_eq[of p, symmetric] Cons(1) sorry
-    qed
-    moreover have "poly.coeff p (m * n) = nth_default 0 (rev (root_poly'_impl n cs) @ [c]) m" 
-      if "n dvd length cs + 1" 
-    proof -
-      have two: "nth_default 0 (root_poly'_impl n cs) n = poly.coeff (root_poly' n (Poly cs)) n" 
-        using 2(1)[OF that]
- sorry
-      show ?thesis sorry
-    qed
-    ultimately show ?case unfolding c[symmetric] by auto 
+  have nth: "rev (root_poly'_impl n (rev (coeffs p))) ! m = poly.coeff p (m*n)" 
+    if "m*n < length (coeffs p)" "p\<noteq>0" using that 
+  proof -
+    have one: "m < length (root_poly'_impl n (rev (coeffs p)))" 
+    by (smt (verit, best) One_nat_def Suc_lessD assms div_less_iff_less_mult div_mult_self_is_m 
+      dvdE length_rev length_root_poly'_impl mult.commute not_less_eq that(1))
+    have two: "m * n < length (rev (coeffs p))" using that by auto
+    have three: "length (rev (coeffs p)) - Suc (m * n) < length (coeffs p)" using that(1) by auto
+    have index: "length (coeffs p) - Suc (length (rev (coeffs p)) - Suc (m * n)) = m*n"
+      by (simp add: Suc_diff_Suc order_less_imp_le that(1))
+    show ?thesis by (subst rev_nth[OF one], subst root_poly'_impl_nth_length[OF \<open>1<n\<close> two], 
+      subst rev_nth[OF three], subst index, intro nth_coeffs_coeff) (use that in \<open>auto\<close>)
   qed
-next
-  case 2
-  then show ?case  sorry
-qed
 
-*)
+  have not_p0: ?case if "p\<noteq>0" unfolding * nth_default_strip_while_dflt
+  unfolding nth_default_def proof (split if_splits, safe, goal_cases)
+    case 1
+    then have mn_len: "m*n < length (coeffs p)"
+    by (smt (verit) assms div_less_iff_less_mult div_mult_self_is_m dvd_triv_right length_rev 
+      length_root_poly'_impl less_numeral_extra(1) linorder_neqE_nat not_less_eq order_less_not_sym 
+      order_less_trans)
+    then show ?case using nth[OF mn_len that, symmetric] 1 by auto
+  next
+    case 2
+    then have mn_len: "m*n \<ge> length (coeffs p)"
+    by (smt (verit, ccfv_SIG) assms div_less_iff_less_mult dvd_div_mult_self length_rev 
+      length_root_poly'_impl less_numeral_extra(1) linorder_not_le nat_neq_iff not_less_eq 
+      order_less_trans)
+    then show ?case using that by (simp add: coeff_eq_0 length_coeffs_degree)
+  qed
+
+  show ?case by (cases "p =0")(use p0 not_p0 in \<open>auto\<close>)
+qed auto
+
 
 
 
@@ -154,10 +189,9 @@ shows "poly.coeff p n = poly.coeff (root_poly' CARD('e) p) (n div CARD('e))"
 proof -
   let ?A = "{x. poly.coeff p (x * CARD('e)) \<noteq> 0}"
   let ?f = "(\<lambda>x. if CARD('e) dvd x then x div CARD('e) else degree p + 1)"
-  have card: "degree p < CARD('e) + degree p * CARD('e)" 
-  by (metis add_gr_0 arithmetic_simps(79) bot_nat_0.not_eq_extremum 
-    linordered_comm_semiring_strict_class.comm_mult_strict_left_mono nontriv trans_less_add2 
-    zero_less_card_finite)
+  have card: "degree p < CARD('e) + degree p * CARD('e)"
+  by (metis One_nat_def Suc_lessI antisym_conv3 less_add_same_cancel2 less_zeroE 
+    n_less_n_mult_m nat_mult_1_right pos_add_strict zero_less_card_finite)
   have "?f -` ?A \<subseteq> {x. poly.coeff p x \<noteq> 0}" using coeff_eq_0[OF card] by auto
   then have f1: "finite (?f -` ?A)" if "finite {x. poly.coeff p x \<noteq> 0}"
     using finite_subset that by blast 
